examples/dsls/mini_steel/Pulse.Elaborate.fsti
@@ -35,3 +35,6 @@ val elab_comp_open_commute (c:comp) (x:term)
 val elab_ln (t:term) (i:int)
   : Lemma (requires ln' t i)
           (ensures RT.ln' (elab_term t) i)
+
+val elab_freevars (e:term)
+  : Lemma (freevars e == RT.freevars (elab_term e))
